theories/noimport/doc/cpp/logic.v
@@ -72,7 +72,7 @@ Example e8 : Rep := longlongR q z. (** similarly, [ulonglongR] and [slonglongR] 
 Example e9 : Rep  := i8R q z. (** similarly, [int16], [int32], [uni64]. Prefix 'u' for the unsigned variants *)
 Variable b: bool.
 Example e11: bool:=true.
-Example e10 : Rep := boolR (cqp.mk false (1/2)%Qp) b.
+Example e10 : Rep := boolR (CV.m (1/2)) b.
 
 (**
 Some locations (e.g. the "next" field of linked list) store pointers.
@@ -117,10 +117,10 @@ Lemma l1: e13 |-- [| False |].
 Abort.
 
 (** However, the following is fine: *)
-Example e14 : mpred := x |-> intR ((cqp.mk false (1/2)%Qp)) 4 ** x |-> intR ((cqp.mk false (1/2)%Qp)) 4.
+Example e14 : mpred := x |-> intR ((CV.m (1/2))) 4 ** x |-> intR ((CV.m (1/2))) 4.
 
 (** if [x] and [y] are different locations, the following is also fine *)
-Example e15 : mpred := x |-> intR 1 4 ** y |-> intR ((cqp.mk false (1/2)%Qp)) 4.
+Example e15 : mpred := x |-> intR 1 4 ** y |-> intR (CV.m (1/2)) 4.
 
 (** This separateness part of the [**] (instead of vanilla conjunction) gives the main modularity properties of separation logic.
 For example, if a thread [t1] has precondition [P1] and postcondition [Q2],
